src/Examples/Interval/Example_Interval_DG_IP_Flagship.thy
@@ -27,7 +27,7 @@ text \<open>
 
 definition twice_program :: imp_prog where
   "twice_program = program {
-     void twice(p) { return p + p }
+     int32 twice(int32 p) { return p + p }
      void main() { x := twice(3); y := twice(10) }
    }"
 
@@ -307,7 +307,7 @@ subsection \<open>Source-level soundness\<close>
 lemma twice_wf: "wf_compile_input twice_gs twice_pi twice_procs (STR ''main'') twice_main"
   unfolding wf_compile_input_simps
     twice_pi_def twice_procs_def twice_main_def twice_program_def
-  by (auto simp: proc_decl_of_def prog_main_name_def valid_formal_def reserved_ret_var_def
+  by (auto simp: proc_decl_of_def proc_decl_of_typed_def prog_main_name_def valid_formal_def reserved_ret_var_def
       value_providing_def source_exp_def ret_var_def
       special_table_def special_pname_nondet_int_def
       special_pname_min_def special_pname_max_def
